Update backend/semantics for new Test

compiler/backend/semantics/dataSemScript.sml
@@ -723,6 +723,13 @@ Definition do_word_app_def:
         | SOME (w1,w2) => SOME (Number &(w2n (opw_lookup opw w1 w2))))) /\
   do_word_app (WordOpw W64 opw) [Word64 w1; Word64 w2] =
         SOME (Word64 (opw_lookup opw w1 w2)) /\
+  do_word_app (WordTest W8 test) [Number n1; Number n2] =
+       (if 0 ≤ n1 ∧ n1 < 256 ∧ 0 ≤ n2 ∧ n2 < 256 then
+          (case test of
+           | Equal => SOME (Boolv (n1 = n2))
+           | Less => SOME (Boolv (n1 < n1))
+           | _ => NONE)
+        else NONE) /\
   do_word_app (WordShift W8 sh n) [Number i] =
        (case some (w:word8). i = &(w2n w) of
         | NONE => NONE
@@ -868,6 +875,10 @@ Definition do_app_aux_def:
              then Rval (EL n xs, s)
              else Error)
          | _ => Error)
+    | (BlockOp (BoolTest test),[v1;v2]) =>
+        (if (v1 ≠ Boolv T ∧ v1 ≠ Boolv F) then Error else
+         if (v2 ≠ Boolv T ∧ v2 ≠ Boolv F) then Error else
+           Rval (Boolv (v1 = v2), s))
     | (BlockOp ListAppend,[x1;x2]) =>
         (case (v_to_list x1, v_to_list x2) of
          | (SOME xs, SOME ys) =>
