compiler/backend/flatLangScript.sml
@@ -33,6 +33,7 @@ Datatype:
   | Opw word_size opw
   | Shift word_size shift num
   | Equality
+  | Test test prim_type
   (* FP operations *)
   | FP_cmp fp_cmp
   | FP_uop fp_uop
