compiler/backend/flat_to_closScript.sml
@@ -150,6 +150,12 @@ Definition compile_op_def:
     | CopyAw8Aw8 => Let t xs (CopyByteAw8 t)
     | Aw8xor_unsafe => Op t (MemOp XorByte) xs
     | VfromList => Op t (BlockOp (FromList 0)) xs
+    | Test test test_ty =>
+         (case test_ty of
+          | BoolT => Op t (BlockOp (BoolTest test)) xs
+          | CharT => Op t (WordOp (WordTest W8 test)) xs
+          | WordT W8 => Op t (WordOp (WordTest W8 test)) xs
+          | _ => Op t (BlockOp Equal) xs)
     | WordFromInt W64 => Op t (WordOp WordFromInt) xs
     | WordToInt W64 => Op t (WordOp WordToInt) xs
     | WordFromInt W8 => arg1 xs (\x. Op t (IntOp Mod) [Op t (IntOp (Const 256)) []; x])
